let rec fact n = match n with 0 -> 1
  | n -> n * fact (n - 1)

let rec fact_aux x n = match n with 0 -> x
  | n -> fact_aux (n * x) (n - 1)

let fact_iter = fact_aux 1



Base Case n=0;


          fact 0
   (fact) = 








          e_1
(rule 1) = e_2
(rule 2) = e_3

(rule n) = e_n


__________________________
Generalized statement (*) (if necessary): <...>
---
Base Case:
Statement being proven in base case: <...>
Proof of base case:
<...>
---
Inductive Step:
Induction hypothesis (or hypotheses): <...>
Statement being proved in inductive step: <...>
Proof of inductive step:
<...>
---
Instantiation of generalization (if necessary):
<...>
---
QED
____________________________
```ocaml
let rec fold_left f acc l =
  match l with [] -> acc | h :: t -> fold_left f (f acc h) t

let rec fold_right f l acc =
  match l with [] -> acc | h :: t -> f h (fold_right f t acc)

let rec map f l =
  match l with [] -> [] | h :: t -> f h :: map f t

let rec nlen n l =
  match l with [] -> 0 | h :: t -> n + nlen n t

let rec len_tr acc l = 
  match l with [] -> acc | _ :: t -> len_tr (acc + 1) t





```
2. Show that the statement

    ```ocaml
    fold_right (fun e a -> g e :: a) l []   =   map g l
    ```

    holds for all Lists l and functions g.
  
Generalized statement (*) (if necessary):  fold_right (fun e a -> g e :: a) l []   =   map g l
---
Base Case: l = []
Statement being proven in base case:   fold_right (fun e a -> g e :: a) [] []   =   map g []
Proof of base case:
                fold_right (fun e a -> g e :: a) [] []
(fold_right)  = match [] with [] -> acc | h :: t -> (fun e a -> g e :: a) h (fold_right (fun e a -> g e :: a) t acc)

(match) = []
        = []
(map)   = match [] with [] -> [] | h :: t -> f h :: map f t
        = map g []
---
Inductive Step:
Induction hypothesis (or hypotheses): 
```ocaml
fold_right (fun e a -> g e :: a) l []   =   map g l
```
Statement being proved in inductive step: 
```ocaml
fold_right (fun e a -> g e :: a) (x::l) []   =   map g (x::l)
```
Proof of inductive step:
              fold_right (fun e a -> g e :: a) (x::l) []
 (fold_right) = match l with [] -> acc | h :: t -> (fun e a -> g e :: a) h (fold_right (fun e a -> g e :: a) t acc)
 (match)      = (fun e a -> g e :: a) x (fold_right (fun e a -> g e :: a) l [])
 (fun)        =  g x :: (fold_right (fun e a -> g e :: a) l [])
              =
(I.H.)        = g x :: (fold_right (fun e a -> g e :: a) l [])
(match)       = g x :: map g l
(map)         = match (x::l) with [] -> [] | h :: t -> g h :: map g t
              map g (x::l)
---
QED

4. Show that the statement

    ```ocaml
    fold_left (fun acc _ -> acc + 1) 0 l   =   len_tr 0 l
    ```

    holds for all Lists l.

Generalized statement (*) (if necessary):fold_left (fun acc _ -> acc + 1) acc []   =   len_tr acc []
---
Base Case: l = []
Statement being proven in base case: 
```ocaml
    fold_left (fun acc _ -> acc + 1) acc []   =   len_tr acc []
```
Proof of base case:

                   fold_left (fun acc _ -> acc + 1) acc []
  (fold_left)      =  match [] with [] -> acc | h :: t -> fold_left (fun acc _ -> acc + 1) ((fun acc _ -> acc + 1) 0 h) t
  (match)          = acc

        (match)    = acc 
        (len_tr)   = match [] with [] -> acc | _ :: t -> len_tr (acc + 1) t
                    len_tr acc []

---
Inductive Step:
Induction hypothesis (or hypotheses): fold_left (fun acc _ -> acc + 1) acc l   =   len_tr acc l
Statement being proved in inductive step: l = x::l
Proof of inductive step:
fold_left (fun acc _ -> acc + 1) acc x::l
(fold_left)  =   match x::l with [] -> acc | h :: t -> fold_left (fun acc _ -> acc + 1) ((fun acc _ -> acc + 1) acc h) t
(match)     = fold_left (fun acc _ -> acc + 1) ((fun acc _ -> acc + 1) acc x) l
(fun )      = fold_left (fun acc _ -> acc + 1) (acc + 1) l
(I.H)       =  len_tr (acc + 1) l


(match)        = len_tr (acc + 1)  l
(len_tr)       = match x::l with [] -> acc | _ :: t -> len_tr (acc + 1) t
len_tr acc x::l







---
Instantiation of generalization (if necessary):
fold_left (fun acc _ -> acc + 1) 0 l 
(*)     = len_tr 0 l
        = len_tr 0 l

QED
5. Show that the statement

    ```ocaml
    nlen n l   =   fold_left (+) 0 (map (fun _ -> n) l)
    ```

    holds for all Lists l.

Generalized statement (*) (if necessary): <...>
---
Base Case: l = []
Statement being proven in base case: 
```ocaml
    nlen n []   =   fold_left (+) 0 (map (fun _ -> n) [])
    ```
Proof of base case:
           nlen n [] 
    (nlen) = match [] with [] -> 0 | h :: t -> n + nlen n t
    (match)= 0
(match)    = 0
(fold_left)=match [] with [] -> 0 | h :: t -> fold_left (+) ((+) 0 h) t
(match)    = fold_left (+) 0 [] 
(map)      = fold_left (+) 0 (match [] with [] -> [] | h :: t -> (fun _ -> n) h :: map (fun _ -> n) t)
            fold_left (+) 0  (map (fun _ -> n) [])

---
Inductive Step:
Induction hypothesis (or hypotheses): 
```ocaml
    nlen n l   =   fold_left (+) 0 (map (fun _ -> n) l)
    ```
Statement being proved in inductive step: 
```ocaml
    nlen n (x::l)   =   fold_left (+) 0 (map (fun _ -> n) (x::l))
    ```
Proof of inductive step:
              nlen n (x::l)
     (nlen)   =  match (x::l) with [] -> 0 | h :: t -> n + nlen n t
     (match)  = n + nlen n l
     (I.H.)   = n + fold_left (+) 0 (map (fun _ -> n) l)



(+)           = fold_left (+) x l
(match)       = fold_left (+) ((+) 0 x) l
  (fold_left) = match (x::l) with [] -> 0 | h :: t -> fold_left (+) ((+) 0 h) t


  (fun)       = fold_left (+) 0 (n :: map (fun _ -> n) l)
  (match)     = fold_left (+) 0 ((fun _ -> n) x :: map (fun _ -> n) l)
  (map)       = fold_left (+) 0 (match (x::l) with [] -> [] | h :: t -> (fun _ -> n) h :: map (fun _ -> n) t)
              fold_left (+) 0 (map (fun _ -> n) (x::l))
---
Instantiation of generalization (if necessary):
<...>
---
QED
___comments__________
(fold_left)   = match l with [] -> x | h :: t -> fold_left (+) ((+) x h) t
______
6. Show that the statement

   ```ocaml
   fold_left (+) 0 l   =   fold_right (+) l 0
   ```

   holds for all Lists l.
7. Consider the following functions

   ```ocaml
   let rec fac n = if n < 1 the 1 else n * fac (n-1)

   let rec facc_help f n =
     if n <= 0 then f 1
     else facc_help (fun p -> f (n*p)) (n-1)

   let facc n = 
     facc_help (fun x -> x) n
   ```

   Show that the statement

   ```ocaml
   facc n   =   fac n
   ```

   for all non negative n.
   Hint: You didnt learn a rule for *if-then-else*, but you can invent one yourself. If you want you can also
   rewrite it to a match expression and use the known rule for that.
8. Do the third exercise on Equational Reasoning [w12t03](https://artemis.ase.in.tum.de/courses/253/exercises/10312)
9. Consider the following function:

   ```ocaml
   let comp f g x = f (g x)
   ```

   Show that the statement

    ```ocaml
    map (cmp f g) l   =   comp (map f) (map g) l
    ```

    holds for all Lists l as well as all functions g and f.

10. Consider the following function:

    ```ocaml
    let app l1 l2 = 
      match l1 with [] -> l2 | h :: t -> h :: app t l2
    ```

    Show that the statement

    ```ocaml
    fold_left (fun a e -> app a [g e]) [] l   =   map g l
    ```

    holds for all Lists l and functions g.\
    Hint: If you manage to do this, then you are waaaayyy more prepared, than you need to be.




______________________
w12t1
```ocaml
let rec fact n = match n with 0 -> 1
  | n -> n * fact (n - 1)

let rec fact_aux x n = match n with 0 -> x
  | n -> fact_aux (n * x) (n - 1)

let fact_iter = fact_aux 1
```

fact_iter n = fact n

Generalized statement (*) (if necessary): <...>
---
Base Case: n = 0
Statement being proven in base case: fact_iter 0 = fact 0
Proof of base case:

              fact_iter 0
  (fact_iter) = fact_aux 1
  (fact_aux)  = match n with 0 -> x | n -> fact_aux (n * x) (n - 1)
  (match)     = 1
 
  (match)     = 1
  (fact)      = match 0 with 0 -> 1 | n -> n * fact (n - 1)
              fact 0

---
Inductive Step: 
Induction hypothesis (or hypotheses): 
fact_iter n = fact n
Statement being proved in inductive step: 
fact_iter (n+1) = fact (n+1)
Proof of inductive step:
              fact_iter (n+1)
  (fact_iter) = fact_aux 1 (n+1)
  (fact_aux)  = match (n+1) with 0 -> x | n -> fact_aux (n * x) (n - 1)
  (match)     = fact_aux ((n+1) * 1) ((n+1) - 1)
  (arith)     = fact_aux (n+1) n


(I.H.)        = (n+1) * fact_iter n 
 (arith)      = (n+1) * fact n
(match)       = (n+1) * fact ((n+1) - 1)
 (fact)       = match (n+1) with 0 -> 1 | n -> n * fact (n - 1)
              = fact (n+1)
---
Instantiation of generalization (if necessary):
<...>
---

QED
